pulse/src/syntax_extension/PulseSyntaxExtension.Sugar.fst
@@ -188,6 +188,13 @@ and let_init =
   | Lambda_initializer of fn_defn
   | Stmt_initializer of stmt
 
+type fn_decl = {
+  id:ident;
+  binders:binders;
+  ascription:either computation_type (option A.term); (* always Inl for now *)
+  range:rng
+}
+
 let tag_of_stmt (s:stmt) : string =
   match s.s with
   | Open _ -> "Open"
@@ -207,6 +214,7 @@ let tag_of_stmt (s:stmt) : string =
 
 type decl =
   | FnDefn of fn_defn
+  | FnDecl of fn_decl
   
 (* Convenience builders for use from OCaml/Menhir, since field names get mangled in OCaml *)
 let mk_comp tag precondition return_name return_type postcondition opens range = 
@@ -232,7 +240,8 @@ let mk_while guard id invariant body = While { guard; id; invariant; body }
 let mk_intro vprop witnesses = Introduce { vprop; witnesses }
 let mk_sequence s1 s2 = Sequence { s1; s2 }
 let mk_stmt s range = { s; range }
-let mk_fn_defn id is_rec binders ascription measure body range = { id; is_rec; binders; ascription; measure; body; range }
+let mk_fn_defn id is_rec binders ascription measure body range : fn_defn = { id; is_rec; binders; ascription; measure; body; range }
+let mk_fn_decl id binders ascription range : fn_decl = { id; binders; ascription; range }
 let mk_open lid = Open lid
 let mk_par p1 p2 q1 q2 b1 b2 = Parallel { p1; p2; q1; q2; b1; b2 }
 let mk_proof_hint_with_binders ht bs =  ProofHintWithBinders { hint_type=ht; binders=bs }
