pulse/src/checker/Pulse.Syntax.Builder.fst
@@ -62,4 +62,5 @@ let mk_fold_hint_type names p = FOLD { names; p }
 let mk_rename_hint_type pairs goal tac_opt = RENAME { pairs; goal; tac_opt=map_opt tac_opt thunk }
 let mk_rewrite_hint_type t1 t2 tac_opt = REWRITE { t1; t2; tac_opt=map_opt tac_opt thunk }
 let mk_fn_defn id isrec bs comp meas body : decl' = FnDefn { id; isrec; bs; comp; meas; body }
+let mk_fn_decl id bs comp : decl' = FnDecl { id; bs; comp; }
 let mk_decl d range : decl = {d; range}
